proof fully complete

LovaszExp.v
@@ -15,8 +15,8 @@ Section GraphExp.
   Context { A B:ordType }.
 
   Definition Exp_of (G: @UG A) (G': @UG B)(g:B-> A):=
-    (nodes G = img g G') /\ (forall x y, x <>y -> g x = g y -> edg G' x y) /\
-    (forall x y, g x <> g y -> edg G (g x) (g y) = edg G' x y).
+    (nodes G = img g G') /\ (forall x y,  In x G' -> In y G'-> x <>y -> g x = g y -> edg G' x y) /\
+    (forall x y, In x G' -> In y G'-> g x <> g y -> edg G (g x) (g y) = edg G' x y).
 
 End GraphExp.
 
@@ -34,10 +34,11 @@ Section ExpProp.
   Lemma exp_elim1a: Exp_of G G' g  -> (img g G' = nodes G).
   Proof. intros h; symmetry; apply h. Qed.
 
-  Lemma exp_elim2 (x y: B): Exp_of G G' g -> x <> y -> g x = g y -> edg G' x y.
+  Lemma exp_elim2 (x y: B): Exp_of G G' g -> In x G' -> In y G'-> x <> y -> g x = g y -> edg G' x y.
   Proof. intros h; apply h. Qed.
 
-  Lemma exp_elim3 (x y: B): Exp_of G G' g -> g x <> g y -> edg G (g x) (g y) = edg G' x y.
+  Lemma exp_elim3 (x y: B): Exp_of G G' g -> In x G' -> In y G'->
+                            g x <> g y -> edg G (g x) (g y) = edg G' x y.
   Proof. intros h; apply h. Qed.
 
   Hint Resolve exp_elim1 exp_elim1a exp_elim2 exp_elim3: core.
@@ -50,7 +51,7 @@ Section ExpProp.
            { assert (h4: x <> y).
              { intro h4;subst x. absurd (edg G' y y);auto. }
              right. replace (edg G (g x) (g y)) with (edg G' x y).
-             auto. symmetry;auto. } } Qed.
+             auto. symmetry;apply h1;eauto. } } Qed.
 
   Lemma exp_intro (x1 x2: A):
     Exp_of G G' g -> edg G x1 x2 -> (exists y1 y2,  ( x1 = g y1 /\ x2 = g y2) /\ edg G' y1 y2 ).
@@ -83,7 +84,6 @@ Section LovaszExp.
 
   Context { A B :ordType }.
   
-  Variable db : B.
 
   Lemma LovaszExpLemma (G: @UG A)(G': @UG B)(g: B-> A): Exp_of G G' g -> Perfect G -> Perfect G'.
   Proof.
@@ -100,15 +100,31 @@ Section LovaszExp.
 
       specialize (forall_xy_EM P G') as HC.
 
+       assert (H_nil: nodes G' = nil \/ nodes G' <> nil).
+        { destruct (nodes G') eqn: hN'. left;auto. right.
+          intro h3. inversion h3. }
+
+        destruct H_nil as [h_nil | h_not_nil].
+        apply nil_is_perfect; auto.
+
+        assert (H: exists c, In c G').
+        {  destruct (nodes G') eqn: hN'.
+           absurd (@nil A = @nil A); auto.
+           exists e. auto. }
+        destruct H as [c H].
+        
+
       (* The proof is split into two cases C1 and C2. 
          C1: forall x y, In x G' -> In y G' -> x<> y -> g x <> g y 
          C2: exists x y, In x G' /\ In y G' /\ x<> y /\ g x = g y   *)
-      destruct HC as [C1 | C2].
+      destruct HC as [C1 | C2]. 
       { (* C1: forall x y, In x G' -> In y G' -> x<> y -> g x <> g y *)
         assert (C1a: forall x y: B, In x G' -> In y G' -> g x = g y -> x = y).
         { intros x y hx hy. specialize (C1 x y hx hy) as hP. unfold P in hP.
           move /impP in hP. intros h3; apply /eqP; apply hP; auto. }
 
+       
+       
         (* In this case G and G' are isomorphic and hence G' is perfect *)
         assert (Hiso: iso G G').
         { apply iso_sym. apply iso_intro with (f:=g). eauto.
@@ -122,7 +138,7 @@ Section LovaszExp.
             { subst x.
               replace (edg G' y y) with false. replace (edg G (g y) (g y)) with false.
               auto. all: symmetry;switch;auto. }
-            { symmetry. apply h1. auto. } }
+            { symmetry. apply h1; auto. } }
           { (*----one_one_on G' g ---*)
             unfold one_one_on; intros;auto. }   }  eauto.  }
 
@@ -141,30 +157,97 @@ Section LovaszExp.
            to IH G'_a' is also perfect. Furthermore, due to LovaszRepLemma G' is also perfect. *)
         destruct C2a as [a C2a]. destruct C2a as [a' C2a].
         set (G'_a':= ind_at (rmv a' G') G').
+        
+        assert (h_rmv: rmv a' G' [i] G' = rmv a' G').
+        { symmetry; apply set_inter_elim15; auto. }
+
+        assert (h_a: In a (rmv a' G')).
+        {  cut (In a G'). cut (a <> a'). auto. all: apply C2a. }
+        
+        assert (h_img: img g G'_a' = img g G').
+        { simpl. rewrite h_rmv. apply set_equal. all: auto.
+          split.
+          { cut ( rmv a' G' [<=] G'). auto. auto. }
+          { intros y h3.
+            assert (h4: exists x, In x G' /\ y = g x). auto.
+            destruct h4 as [x h4]. destruct h4 as [h4a h4].
+            assert (h5: x = a' \/ x <> a'). eauto.
+            destruct h5 as [h5 | h5].
+            {  subst x;subst y. replace (g a') with (g a). auto.
+               apply C2a. }
+            { subst y. cut (In x (rmv a' G')). auto. auto. } } }             
+        
         assert (hsize: | G'_a'| < |G' |).
-        { simpl. replace (rmv a' G' [i] G') with (rmv a' G').
+        { simpl. rewrite h_rmv.
           replace (| rmv a' G' |) with (|G'| - 1).
           cut (|G'| > 0). omega. cut (In a G').
           case (nodes G'). simpl. tauto. intros;simpl;auto;omega. apply C2a.
-          symmetry; eapply rmv_card1;apply C2a.
-          apply set_inter_elim15; auto. }
+          symmetry; eapply rmv_card1;apply C2a.  } 
 
-        assert (h3: Exp_of G G'_a' g). admit.
+        assert (h3: Exp_of G G'_a' g).
+        { unfold Exp_of. rewrite h_img.
+          split. apply h1.
+          split. 
+          { intros x y h3 h4 h5 h6. replace (edg G'_a' x y) with (edg G' x y).
+            apply h1; subst G'_a'; simpl in h3, h4; eauto.
+            unfold G'_a'. auto. }
+          { intros x y h3 h4 h5. replace (edg G'_a' x y) with (edg G' x y).
+            apply h1; subst G'_a'; simpl in h3, h4; eauto.
+            unfold G'_a'. auto. } }
 
-        assert (h4: Perfect G'_a'). admit.
+        assert (h4: Perfect G'_a').
+        { apply IH;auto. }
 
-        assert (h5: Rep_in G'_a' a a' G'). admit.
-
+        assert (h5: Rep_in G'_a' a a' G').
+        { unfold Rep_in. subst G'_a'. simpl. rewrite h_rmv.
+          split.
+          { cut (In a G'). cut (a <> a'). auto. all: apply C2a. }
+          split.
+          { cut (NoDup G'). auto. eauto. }
+          split.
+          { apply rmv_add. auto. apply C2a. }
+          split.
+          { unfold Exp_of in h1. apply h1. all: apply C2a. }
+          split.
+          { intros x y h5 h6.  symmetry; auto. }
+          { intros x h5. unfold Exp_of in h1.
+            assert (h6: In x G' \/ ~ In x G'). eauto.
+            assert (hG_G': nodes G' = add a' (rmv a' G')).
+            { apply rmv_add. auto. apply C2a. }
+            assert (ha: In a (rmv a' G')).
+            { cut (In a G'). cut (a <> a'). auto. all: apply C2a. } 
+            destruct h6 as [h6 | h6].
+            { (*- In x G' --*)
+              assert (h7: x = a' \/ In x (rmv a' G')).
+              { rewrite hG_G' in h6. auto. }
+              destruct h7 as [h7 |h7].
+              { subst x. replace (edg G' a' a') with false.
+                switch. cut (~ In a' (rmv a' G')).
+                intros h7 h8; apply h7; eauto.
+                cut (NoDup G'); auto. symmetry;switch;auto. }
+              { replace ((edg G' at_ rmv a' G') x a) with (edg G' x a).
+                Focus 2. by auto.
+                assert (h8: g x = g a \/ g x <> g a). eauto.
+                destruct h8 as [h8 | h8].
+                { replace (edg G' x a) with true.
+                  symmetry. apply h1. all: auto.
+                  apply C2a. intro h9. subst x.
+                  absurd (In a' (rmv a' G')). cut (NoDup G'); auto. auto.
+                  rewrite h8;apply C2a.
+                  symmetry; apply h1. all: auto. apply C2a. }
+                { assert (h9: g a = g a'). apply C2a.
+                  replace (edg G' x a) with (edg G (g x) (g a)).
+                  rewrite h9. apply h1. all: auto. apply C2a.
+                  rewrite <- h9;auto.
+                  apply h1. all: auto. apply C2a. } } }
+            { (*- ~ In x G' --*)
+              replace (edg G' x a') with false.
+              Focus 2.  symmetry;switch; intro h8;apply h6;eauto.
+              switch. intro h8;apply h6.
+              cut (In x (rmv a' G')). eauto. eauto. } } }
+              
+            
         eapply ReplicationLemma. exact h4. exact h5. }    } Qed.
        
-       
-      
-          
-
-  
-  
-
-  
- 
-    
+           
   End LovaszExp.
